checkpoint diamond property

src/theory/bir/bir_promising_diamondScript.sml
@@ -1,6 +1,57 @@
-
-  
+open HolKernel Parse;
+open bir_promisingTheory;
+open pred_setTheory;
+open finite_setTheory;
 
 val _ = new_theory "bir_promising_diamond";
+
+Definition bir_promising_sim_rel_def:
+  sim_rel (cores:core_t -> bool,M:mem_msg_t list) (cores',M') =
+   (rel_set $= cores cores' /\ M = M')
+End
+
+Definition bir_promise_step_def:
+  promise_step (cores,M) (cores',M') =
+     (parstep cores M cores' M' /\ ~(M = M'))
+End
+
+Definition bir_nonpromise_step_def:
+  nonpromise_step (cores,M) (cores',M') =
+  (parstep cores M cores' M' /\ (M = M'))
+End
+
+Triviality sim_rel_eq:
+  sim_rel (cores,M) (cores',M') = (cores = cores' /\ M = M')
+Proof
+  fs[bir_promising_sim_rel_def]
+QED
+
+Theorem promise_inversion:
+  parstep cores M cores' M' /\ ~(M = M')
+==>
+  ∃p cid s s' prom msg.
+  cores' = cores DIFF {core cid p s} ∪ {core cid p s'} ∧ core cid p s ∈ cores ∧
+  is_certified p cid s' M' ∧
+  msg.cid = cid ∧ prom = LENGTH M + 1 ∧ s' = s with bst_prom updated_by (\pr. pr ++ [prom]) ∧
+  M' = M ++ [msg]
+Proof
+  fs[bir_parstep_cases, bir_cstep_cases]
+QED
+
+Theorem bir_promising_diamond:
+  !T1 T2 T3 M1 M2 M3.
+  (nonpromise_step (T1,M1) (T2,M2) /\ promise_step (T2,M2) (T3,M3))
+  ==>
+  ?T1' T2' T3' M1' M2' M3'.
+       sim_rel (T1,M1) (T1',M1')
+    /\ promise_step (T1',M1') (T2',M2')
+    /\ nonpromise_step (T2',M2') (T3',M3')
+    /\ sim_rel (T3,M3) (T3',M3')
+Proof
+  REWRITE_TAC[bir_nonpromise_step_def, bir_promise_step_def]
+>> REPEAT STRIP_TAC
+>> fs[sim_rel_eq]
+>> cheat
+QED
 
 val _ = export_theory ()
